theories/backtranslations/st_sem/correctness/help.v
@@ -1,0 +1,46 @@
+From iris.program_logic Require Import lifting ectx_lifting.
+From st.lamst Require Import lang.
+
+Definition fresh_loc (σ : gmap loc val) : loc :=
+  fresh (dom (gset loc) σ).
+
+Lemma fresh_loc_lookup_None (σ : gmap loc lamst.lang.val) :
+  σ !! fresh_loc σ = None.
+Proof.
+  rewrite /fresh_loc.
+  by apply (not_elem_of_dom (D := gset loc)), is_fresh.
+Qed.
+
+Lemma inv_prim_step_Compare_locs (l1 l2 : loc) e2 (σ1 σ2 : state) κ efs (Hstep : prim_step (Compare l1 l2) σ1 κ e2 σ2 efs) :
+  κ = [] ∧ efs = [] ∧ e2 = (bool_decide (l1 = l2)) ∧ σ1 = σ2.
+Proof.
+  simpl in *.
+  assert (efs = []) as ->. by eapply ST_step_no_spawn.
+  assert (κ = []) as ->. by eapply ST_step_no_obs.
+  assert (Hheadstep : head_step (Compare l1 l2) σ1 [] e2 σ2 []). apply (@head_reducible_prim_step lamst_ectx_lang); auto.
+  { exists [], (of_val $ bool_decide (l1 = l2)), σ1, []. simpl.
+    destruct (decide (l1 = l2)) as [<- | neq].
+    + rewrite bool_decide_eq_true_2; auto.
+      apply Compare_suc_head_step.
+    + rewrite bool_decide_eq_false_2; auto.
+      by apply Compare_fail_head_step.
+  }
+  inversion_clear Hheadstep; auto;
+    [by rewrite bool_decide_eq_true_2 | by rewrite bool_decide_eq_false_2].
+Qed.
+
+Lemma pure_step_eq_loc (l1 l2 : loc) : pure_step (Compare l1 l2)%Eₛₜ (of_val $ bool_decide (l1 = l2)).
+Proof.
+  split.
+  - intros σ. rewrite /reducible_no_obs.
+    exists (of_val $ bool_decide (l1 = l2)), σ, [].
+    destruct (decide (l1 = l2)) as [<- | neq].
+    + rewrite bool_decide_eq_true_2; auto. apply head_prim_step.
+      (* Unset Printing Notations. Set Printing Coercions. *)
+      apply Compare_suc_head_step.
+    + rewrite bool_decide_eq_false_2; auto. apply head_prim_step.
+      by apply Compare_fail_head_step.
+  - intros. simpl in H.
+    by destruct (inv_prim_step_Compare_locs _ _ _ _ _ _ _ H) as (-> & -> & -> & ->).
+Qed.
+
