theories/backtranslations/st_sem/correctness/sem_le_st/logrel/fundamental.v
@@ -1,0 +1,55 @@
+From iris Require Import program_logic.weakestpre.
+From iris.proofmode Require Import tactics.
+From iris.base_logic.lib Require Import invariants gen_heap.
+From st.prelude Require Import big_op_three.
+
+From st.lamst Require Import lang types typing.
+From st.lam Require Import lang wkpre.
+
+From st.backtranslations.st_sem Require Import expressions ghost heap_emul.base.
+From st.backtranslations.st_sem.correctness.sem_le_st.logrel Require Import lift definition compat_lemmas.
+
+Section fundamental_theorem.
+
+  Context `{Σ : !gFunctors}.
+  Context `{irisG_inst : !irisG lam_lang Σ}.
+
+  Context `{genHeapG_inst : !gen_heapG loc lamst.lang.val Σ}.
+
+  Context `{val_ghost_mapG_inst : !ghost_mapG Σ nat val}.
+  Context `{loc_ghost_mapG_inst : !ghost_mapG Σ nat loc}.
+
+  Lemma fundamental (Γ : list lamst.types.type) (e : lamst.lang.expr) (τ : lamst.types.type)
+        (d : Γ ⊢ₛₜ e : τ) :
+    open_exprel_typed Γ <<e>> e τ.
+  Proof.
+    induction d; simpl.
+    - admit.
+    - admit.
+    - admit.
+    - admit.
+    - admit.
+    - admit.
+    - admit.
+    - admit.
+    - admit.
+    - admit.
+    - admit.
+    - admit.
+    - admit.
+    - admit.
+    - admit.
+    - admit.
+    - admit.
+    - admit.
+      (* !! intersting ones !! *)
+    - by apply compat_alloc.
+    - by apply compat_read.
+    - apply (compat_write _ _ _ _ _ _ _ IHd1 IHd2). (* "by eapply"; why so long? *)
+    - eapply compat_bind. exact IHd1. exact IHd2.
+    - by apply compat_retrn.
+    - by apply compat_runst.
+    - by eapply compat_compare.
+  Admitted.
+
+End fundamental_theorem.
