theories/backtranslations/st_sem/correctness/st_le_sem/logrel/fundamental.v
@@ -1,0 +1,61 @@
+From iris Require Import program_logic.weakestpre.
+From iris.proofmode Require Import tactics.
+From iris.base_logic.lib Require Import invariants gen_heap.
+
+Local Notation "l ↦ v" := (mapsto l (DfracOwn 1) v)
+  (at level 20, format "l  ↦  v") : bi_scope.
+
+From st.prelude Require Import big_op_three.
+
+From st.lam Require Import lang.
+From st.lamst Require Import wkpre lang types typing.
+
+From st.backtranslations.st_sem Require Import expressions ghost heap_emul.base.
+From st.backtranslations.st_sem.correctness.st_le_sem.logrel Require Import lift definition compat_lemmas.
+
+Section fundamental_theorem.
+
+  Context `{Σ : !gFunctors}.
+
+  Context `{invG_inst : !invG Σ}.
+  Context `{genHeapG_inst : !gen_heapG loc val Σ}.
+
+  Context `{val_ghost_mapG_inst : !ghost_mapG Σ nat lam.lang.val}.
+  Context `{loc_ghost_mapG_inst : !ghost_mapG Σ nat loc}.
+
+  Opaque encode alloc read write bind retrn.
+
+  Lemma fundamental (Γ : list lamst.types.type) (e : lamst.lang.expr) (τ : lamst.types.type)
+        (d : Γ ⊢ₛₜ e : τ) :
+    open_exprel_typed Γ e <<e>> τ.
+  Proof.
+    induction d; simpl.
+    - admit.
+    - admit.
+    - admit.
+    - admit.
+    - admit.
+    - admit.
+    - admit.
+    - admit.
+    - admit.
+    - admit.
+    - admit.
+    - admit.
+    - admit.
+    - admit.
+    - admit.
+    - admit.
+    - admit.
+    - admit.
+      (* !! intersting ones !! *)
+    - by apply compat_alloc.
+    - by apply compat_read.
+    - by eapply compat_write.
+    - by eapply compat_bind.
+    - by apply compat_retrn.
+    - by apply compat_runst.
+    - by eapply compat_compare.
+  Admitted.
+
+End fundamental_theorem.
