theories/backtranslations/st_sem/correctness/st_le_sem/logrel/lift.v
@@ -1,0 +1,61 @@
+From iris Require Import program_logic.weakestpre.
+From iris.proofmode Require Import tactics.
+From iris_string_ident Require Import ltac2_string_ident.
+
+From st.lam Require Import lang.
+From st.lamst Require Import lang wkpre.
+
+Section lift.
+
+  Context `{Σ : !gFunctors}.
+  Context `{irisG_inst : !irisG lamst_lang Σ}.
+
+  Context (s : stuckness).
+
+  Definition lift (Φ : valO -n> lam.lang.valO -n> iPropO Σ) : exprO → lam.lang.exprO → iProp Σ :=
+    fun eᵢ eₛ => (WP eᵢ @ s ; top {{ vᵢ, ∃ vₛ, ⌜ rtc lam_step eₛ (lam.lang.of_val vₛ) ⌝ ∧ Φ vᵢ vₛ }})%I.
+
+  Lemma lift_bind (Kᵢ : list ectx_item) (Kₛ : list lam.lang.ectx_item) (Φ Ψ : valO -n> lam.lang.valO -n> iPropO Σ)
+        (eᵢ : expr) (eₛ  : lam.lang.expr) :
+    ⊢ lift Φ eᵢ eₛ -∗ (∀ vᵢ vₛ, Φ vᵢ vₛ -∗ lift Ψ (fill Kᵢ (of_val vᵢ)) (fill Kₛ (lam.lang.of_val vₛ))) -∗ lift Ψ (fill Kᵢ eᵢ) (fill Kₛ eₛ).
+  Proof.
+    iIntros "HΦeN H". rewrite /lift.
+    iApply wp_bind'. iApply (wp_wand with "HΦeN").
+    iIntros (v). iIntros "des". iDestruct "des" as (v') "[%HNv' Hvv']".
+    iSpecialize ("H" $! v v' with "Hvv'").
+    iApply (wp_wand with "H").
+    iIntros (w). iIntros "des". iDestruct "des" as (w') "[%HKₛv'w' Hww']".
+    iExists w'. iFrame. iPureIntro.
+    apply (rtc_transitive _ (fill Kₛ v')); auto. simpl in *.
+    by apply (rtc_lam_step_ctx (fill Kₛ)).
+  Qed.
+
+  Lemma lift_rtc_steps Φ eᵢ e e' (H : rtc lam_step e e') : lift Φ eᵢ e' ⊢ lift Φ eᵢ e.
+  Proof.
+    iIntros "H". iApply (wp_wand with "H").
+    iIntros (v) "des". iDestruct "des" as (w') "[%H1 H2]". iExists w'. iFrame "H2".
+    iPureIntro. by eapply rtc_transitive.
+  Qed.
+
+  Lemma lift_pure_step_later Φ e e' eₛ (H : pure_step e e') : ▷ lift Φ e' eₛ ⊢ lift Φ e eₛ.
+  Proof. by iApply wp_pure_step_later. Qed.
+
+  Lemma lift_step Φ eᵢ e e' (H : lam_step e e') : lift Φ eᵢ e' ⊢ lift Φ eᵢ e.
+  Proof. iApply lift_rtc_steps. by apply rtc_once. Qed.
+
+  Lemma lift_val (Ψ : valO -n> lam.lang.valO -n> iPropO Σ) vᵢ vₛ : (Ψ vᵢ vₛ) ⊢ lift Ψ vᵢ vₛ.
+  Proof. iIntros "Hv". rewrite /lift. iApply wp_value'. iExists vₛ. auto. Qed.
+
+  Lemma lift_val_fupd (Ψ : valO -n> lam.lang.valO -n> iPropO Σ) vᵢ vₛ : (|={⊤}=> Ψ vᵢ vₛ) ⊢ lift Ψ vᵢ vₛ.
+  Proof. iIntros "Hv". rewrite /lift. iApply wp_value_fupd'. iExists vₛ. iMod "Hv". iModIntro. iSplit; auto. Qed.
+
+  Lemma lift_wand (Φ Ψ : valO -n> lam.lang.valO -n> iPropO Σ) e e' :
+    ⊢ (∀ v v', Φ v v' -∗ Ψ v v') -∗ lift Φ e e' -∗ lift Ψ e e'.
+  Proof.
+    iIntros "H Hee'". rewrite /lift.
+    iApply (wp_wand with "Hee'"). iIntros (v) "Hdes".
+    iDestruct "Hdes" as (v') "[%He'v' HΦ]".
+    iExists v'. iSplit. auto. by iApply "H".
+  Qed.
+
+End lift.
