theories/backtranslations/st_sem/expressions.v
@@ -1,6 +1,6 @@
 From st.lamst Require Import lang.
 From st.lam Require Import lang.
-From st.backtranslations.st_sem Require Import heap.
+From st.backtranslations.st_sem Require Import heap_emul.base.
 
 Reserved Notation "<< e >>" (at level 4, e at next level).
 Fixpoint back_expr (e : lamst.lang.expr) : expr :=
