theories/backtranslations/st_sem/heap_emul/spec.v
@@ -1,0 +1,293 @@
+From iris Require Import program_logic.weakestpre.
+From iris.proofmode Require Import tactics.
+From iris_string_ident Require Import ltac2_string_ident.
+From st.lam Require Import lang wkpre tactics lib.fixlam.
+From st.backtranslations.st_sem Require Import ghost.
+From st.backtranslations.st_sem.heap_emul Require Import base.
+From st.prelude Require Import at_least_one.
+
+Ltac rtc_step := eapply rtc_l; first auto_lam_step; simplify_custom.
+
+(* allocation *)
+
+Lemma alloc_help_spec (vs : list val) (v : val) :
+  rtc lam_step (alloc_help (encode vs) v) (encode (vs ++ [v])).
+Proof.
+  auto_rtc_lam_step. auto_rtc_lam_step.
+  rewrite reverse_snoc app_length /=.
+  auto_rtc_lam_step. assert ((length vs + 1%nat)%Z = S (length vs)) as ->; first lia. apply rtc_refl.
+Qed.
+
+Lemma alloc_v_steps (vs : list val) (v : val) :
+  rtc lam_step
+      (alloc_v v (encode vs))
+      (encode (vs ++ [v]), length vs)%Eₙₒ.
+Proof.
+  rewrite /alloc_v.
+  apply rtc_l with (y := (alloc_help (encode vs) v, Snd (encode vs))%Eₙₒ).
+  apply head_prim_step. eapply App_Lam_head_step'. by asimpl. by rewrite to_of_val.
+  eapply rtc_transitive.
+  apply (rtc_lam_step_ctx (fill [PairLCtx _])).
+  apply alloc_help_spec. simpl.
+  change ((encode_help (reverse (vs ++ [v])), length (vs ++ [v]))%Eₙₒ) with
+      (of_val (encode_help (reverse (vs ++ [v])), length (vs ++ [v]))%Vₙₒ).
+  apply (rtc_lam_step_ctx (fill [PairRCtx _])).
+  rtc_step. apply rtc_refl.
+Qed.
+
+Lemma alloc_step (v : val) : lam_step (alloc v) (alloc_v v).
+Proof.
+  rewrite /alloc /alloc_v.
+  apply head_prim_step. eapply App_Lam_head_step'. by asimpl. by rewrite to_of_val.
+Qed.
+
+(* reading *)
+
+Lemma read_help_spec (vs : list val) (i : nat) (v : val) (piv : vs !! i = Some v) :
+  rtc lam_step (read_help (encode vs) i)%Eₙₒ (v)%Eₙₒ.
+Proof.
+  induction vs as [|last vs IHvs] using rev_ind; try by (exfalso; inversion piv).
+  eapply rtc_transitive. eapply nsteps_rtc. eapply App_Rec_nsteps. by rewrite to_of_val. simplify_custom.
+  do 6 rtc_step;
+  rewrite reverse_snoc; simpl.
+  (* destruct (decide ((1%nat + i)%Z = S (length vs))) as [eq | neq]. *)
+  + (* is equal *)
+    (* rewrite bool_decide_eq_true_2; try done. *)
+    repeat rtc_step.
+    rewrite (list_lookup_middle vs [] last i) in piv; try by lia. inversion piv; try by lia.
+    auto_rtc_lam_step.
+    rewrite app_length /= in H. lia.
+  + (* inductive case *)
+    rewrite app_length /=. rtc_step.
+    assert (i < length (vs ++ [last])). by eapply lookup_lt_Some. rewrite app_length /= in H. rewrite lookup_app_l in piv; try lia. specialize (IHvs piv).
+    eapply rtc_l. apply (lam_step_ctx (fill [AppRCtx _])). auto_lam_step. simplify_custom.
+    eapply rtc_l. apply (lam_step_ctx (fill [AppRCtx _])). auto_lam_step. simplify_custom.
+    assert (S (length vs) - 1%nat = length vs)%Z as ->; try lia.
+    apply IHvs. rewrite app_length /= in H0. lia.
+Qed.
+
+Lemma read_i_steps (vs : list val) (v : val) (i : nat) (H : vs !! i = Some v) :
+  rtc lam_step (read_i i (encode vs)) (encode vs, v)%Vₙₒ.
+Proof.
+  simpl.
+  eapply rtc_l.
+  auto_lam_step. simplify_custom.
+  change ((encode_help (reverse vs), length vs)%Eₙₒ) with
+      (of_val (encode_help (reverse vs), length vs)%Vₙₒ).
+  apply (rtc_lam_step_ctx (fill [PairRCtx _])).
+  by apply read_help_spec.
+Qed.
+
+Lemma read_i_at_least_one (vs : list val) (v : val) (i : nat) (H : vs !! i = Some v) :
+  at_least_one lam_step (read_i i (encode vs)) (encode vs, v)%Vₙₒ.
+Proof.
+  simpl.
+  eapply at_least_one_l.
+  auto_lam_step. simplify_custom.
+  change ((encode_help (reverse vs), length vs)%Eₙₒ) with
+      (of_val (encode_help (reverse vs), length vs)%Vₙₒ).
+  apply (rtc_lam_step_ctx (fill [PairRCtx _])).
+  by apply read_help_spec.
+Qed.
+
+Section wp_read_i.
+
+  Context `{Σ : !gFunctors}.
+  Context `{irisG_inst : !irisG lam_lang Σ}.
+  Context `{ghost_mapG_inst : !ghost_mapG Σ nat (prod val val)}.
+
+  Lemma wp_read_i Φ (vs : list val) (v : val) (i : nat) : ▷ (Φ (encode vs, v)%Vₙₒ ∗ ⌜ vs !! i = Some v ⌝) ⊢ WP read_i i (encode vs) {{Φ}}.
+  Proof.
+    iIntros "H". iApply wp_step_later.
+    auto_lam_step. simplify_custom.
+    iNext. iDestruct "H" as "[H %H]".
+    iApply wp_rtc_steps.
+    change ((encode_help (reverse vs), length vs)%Eₙₒ) with
+        (of_val (encode_help (reverse vs), length vs)%Vₙₒ).
+    apply (rtc_lam_step_ctx (fill [PairRCtx _])).
+    by apply read_help_spec. simpl.
+    change ((encode_help (reverse vs), length vs)%Eₙₒ) with
+        (of_val (encode vs)%Vₙₒ).
+    change ((encode vs, v)%Eₙₒ) with
+        (of_val (encode vs, v)%Vₙₒ).
+    by iApply wp_value'.
+  Qed.
+
+End wp_read_i.
+
+Lemma read_step (i : nat) : lam_step (read i) (read_i i).
+Proof. apply head_prim_step. eapply App_Lam_head_step'. by asimpl. by simpl. Qed.
+
+(* writing *)
+
+Lemma write_help_spec (vs : list val) (i : nat) (v v' : val) (piv : vs !! i = Some v) :
+  rtc lam_step (write_help (encode vs) i v')%Eₙₒ (encode_help (reverse (<[i := v']> vs)))%Eₙₒ.
+Proof.
+  induction vs as [|last vs IHvs] using rev_ind; try by (exfalso; inversion piv).
+  rewrite /encode reverse_snoc. simpl.
+  eapply rtc_transitive. eapply nsteps_rtc. eapply App_Rec_nsteps. simpl. by rewrite !to_of_val /=. do 6 rtc_step.
+  + (* is equal *) repeat rtc_step.
+    rewrite app_length /= in H.
+    rewrite (list_lookup_middle vs [] last i) in piv; try by lia. inversion piv.
+    assert (i = length vs + 0) as ->; first lia. rewrite insert_app_r /= reverse_snoc. apply rtc_refl.
+  + (* inductive case *)
+    assert (i ≠ length vs). rewrite app_length /= in H. lia.
+    assert (i < length (vs ++ [last])). by eapply lookup_lt_Some.
+    assert (i < length vs). rewrite app_length /= in H1. lia.
+    do 4 rtc_step.
+    rewrite lookup_app_l in piv; try lia. specialize (IHvs piv).
+    rewrite (insert_app_l vs [last] i ) /=; try lia. rewrite reverse_snoc /=.
+    apply (rtc_lam_step_ctx (fill [PairRCtx _])).
+    rewrite app_length /=.
+    assert ((length vs + 1)%nat - 1%nat = length vs)%Z as ->; try lia. apply IHvs.
+Qed.
+
+Definition write_i_v_vs (i : expr) (v : expr) (vs : expr) : expr (* : H → H × nat *) :=
+  (((write_help vs i v), (Snd vs)), ())%Eₙₒ.
+
+Lemma write_i_v_step i v (vs : val) :
+  lam_step (write_i_v i v vs) (write_i_v_vs i v vs).
+Proof.
+  apply head_prim_step. eapply App_Lam_head_step'.
+  asimpl. rewrite Rec_subst /write_i_v_vs /write_help. by asimpl. by rewrite to_of_val.
+Qed.
+
+Lemma write_i_v_steps (vs : list val) (i : nat) (v v' : val) (piv : vs !! i = Some v) :
+  rtc lam_step (write_i_v i v' (encode vs)) (encode (<[i := v']> vs), ())%Vₙₒ.
+Proof.
+  rtc_step.
+  apply (rtc_lam_step_ctx (fill [PairLCtx _])).
+  rewrite insert_length.
+  eapply rtc_transitive.
+  apply (rtc_lam_step_ctx (fill [PairLCtx _])).
+  rewrite Rec_subst. asimpl.
+  eapply write_help_spec. done.
+  simpl. rtc_step. apply rtc_refl.
+Qed.
+
+Lemma write_i_v_vs_steps (vs : list val) (i : nat) (v v' : val) (piv : vs !! i = Some v) :
+  rtc lam_step (write_i_v_vs i v' (encode vs)) (encode (<[i := v']> vs), ())%Vₙₒ.
+Proof.
+  rewrite /write_i_v_vs.
+  simpl.
+  apply (rtc_lam_step_ctx (fill [PairLCtx _])).
+  rewrite insert_length.
+  eapply rtc_transitive.
+  apply (rtc_lam_step_ctx (fill [PairLCtx _])).
+  eapply write_help_spec. done.
+  simpl. rtc_step. apply rtc_refl.
+Qed.
+
+Lemma write_i_v_at_least_one (vs : list val) (i : nat) (v v' : val) (piv : vs !! i = Some v) :
+  at_least_one lam_step (write_i_v i v' (encode vs)) (encode (<[i := v']> vs), ())%Vₙₒ.
+Proof.
+  eapply at_least_one_l. auto_lam_step. simplify_custom.
+  apply (rtc_lam_step_ctx (fill [PairLCtx _])).
+  rewrite insert_length.
+  eapply rtc_transitive.
+  apply (rtc_lam_step_ctx (fill [PairLCtx _])).
+  rewrite Rec_subst. asimpl.
+  eapply write_help_spec. done.
+  simpl. rtc_step. apply rtc_refl.
+Qed.
+
+Lemma write_i_step (i : val) (v : val) : lam_step (write_i i v) (write_i_v i v).
+Proof.
+  rewrite /write_i.
+  apply head_prim_step. eapply App_Lam_head_step'.
+  asimpl. rewrite Rec_subst. asimpl. rewrite /write_help. by asimpl.
+  by rewrite to_of_val.
+Qed.
+
+Lemma write_step (i : val) : lam_step (write i) (write_i i).
+Proof.
+  rewrite /write.
+  apply head_prim_step. eapply App_Lam_head_step'.
+  asimpl. rewrite /write_help Rec_subst. asimpl. rewrite /write_help. by asimpl.
+  by rewrite to_of_val.
+Qed.
+
+(* Section wp_write_i_v. *)
+
+(*   Context `{Σ : !gFunctors}. *)
+(*   Context `{irisG_inst : !irisG lam_lang Σ}. *)
+(*   Context `{ghost_mapG_inst : !ghost_mapG Σ nat (prod val val)}. *)
+
+(*   Lemma wp_write_i_v γ Φ (ps : list (val * val)) (v1 v1' v2 v2' : val) (i : nat) : *)
+(*     ⊢ auth_list γ ps -∗ ▷ i ↪[γ] (v1,v1') -∗ *)
+(*       (auth_list γ (<[ i := (v2,v2') ]> ps) -∗ i ↪[γ] (v2,v2') -∗ Φ (encode (<[i := v2]> ps.*1), ())%Vₙₒ) -∗ *)
+(*       WP write_i_v i v2 (encode ps.*1) {{Φ}}. *)
+(*   Proof. *)
+(*     iIntros "Hauth Hi Hu". iApply wp_step_later. auto_lam_step. simplify_custom. iNext. *)
+
+(*   apply (rtc_lam_step_ctx (fill [PairLCtx _])). *)
+(*   rewrite insert_length. *)
+(*   eapply rtc_transitive. *)
+(*   apply (rtc_lam_step_ctx (fill [PairLCtx _])). *)
+(*   rewrite Rec_subst. asimpl. *)
+(*   eapply write_help_spec. done. *)
+(*   simpl. rtc_step. apply rtc_refl. *)
+
+(*     auto_lam_step. simplify_custom. *)
+(*     iNext. iDestruct "H" as "[H %H]". *)
+(*     iApply wp_rtc_steps. *)
+(*     change ((encode_help (reverse vs), length vs)%Eₙₒ) with *)
+(*         (of_val (encode_help (reverse vs), length vs)%Vₙₒ). *)
+(*     apply (rtc_lam_step_ctx (fill [PairRCtx _])). *)
+(*     by apply read_help_spec. simpl. *)
+(*     change ((encode_help (reverse vs), length vs)%Eₙₒ) with *)
+(*         (of_val (encode vs)%Vₙₒ). *)
+(*     change ((encode vs, v)%Eₙₒ) with *)
+(*         (of_val (encode vs, v)%Vₙₒ). *)
+(*     by iApply wp_value'. *)
+(*   Qed. *)
+
+(* End wp_write_i_v. *)
+
+(* monad *)
+
+Lemma retrn_step (v : val) : lam_step (retrn v) (retrn_v v).
+Proof. apply head_prim_step. eapply App_Lam_head_step'. rewrite /retrn_v. by asimpl. by rewrite to_of_val. Qed.
+
+Definition bind_v_f (v f : expr) : val (* : H → H × τ' *):=
+  LamV (* h₀ : H *) (
+      LetIn ((*a*)v.[ren (+1)] (*h₀*)%0) (*h₁v*) (
+              LetIn (Fst %0(*h₁v*)) (*h₁*) (
+                      LetIn (Snd %1) (*v*) (
+                              f.[ren (+4)](*f*) %0(*v*) %1(*h₁*)
+                            )
+                    )
+            )
+    )%Eₙₒ.
+
+
+Lemma bind_step (v : val) : lam_step (bind v) (bind_v v).
+Proof. apply head_prim_step. eapply App_Lam_head_step'. by asimpl. by rewrite to_of_val. Qed.
+
+Lemma bind_v_step (v f : val) : lam_step (bind_v v f) (bind_v_f v f).
+Proof. apply head_prim_step. eapply App_Lam_head_step'. by asimpl. by rewrite to_of_val. Qed.
+
+Lemma bind_v_f_step (v r1 r2 s1 f h0 h1 h2 : lam.lang.val) :
+  rtc lam_step (v h0) (h1, r1)%Eₙₒ →
+  rtc lam_step (f r1) s1 →
+  rtc lam_step (s1 h1) (h2, r2)%Eₙₒ →
+  rtc lam_step (bind_v_f v f h0) (h2, r2)%Eₙₒ.
+Proof.
+  intros H1 H2 H3.
+  rewrite /bind_v_f.
+  rtc_step.
+  eapply rtc_transitive. by apply (rtc_lam_step_ctx (fill_item (LetInCtx _))). simpl.
+  do 5 rtc_step.
+  eapply rtc_transitive. by apply (rtc_lam_step_ctx (fill_item (AppLCtx _))). auto.
+Qed.
+
+(* other *)
+
+Typeclasses Opaque alloc_help.
+Global Opaque alloc_help.
+
+Typeclasses Opaque read_help.
+Global Opaque read_help.
+
+Typeclasses Opaque write_help.
+Global Opaque write_help.
